---
title: 'Exercise 3.1.1c (C3-P1)'
subtitle: 'MATH411'
author: 'Nathan Lunceford'
format:
  html:
    self-contained: true
    page-layout: full
    toc: true
    toc-depth: 1
    toc-location: right
    number-sections: false
    html-math-method: katex
    embed-resources: true
    code-fold: true
    code-summary: 'Show the code'
    code-overflow: wrap
    code-copy: hover
    code-tools:
      source: false
      toggle: true
      caption: See code
engine: jupyter
preview:
  port: 3000
  browser: true
  watch-inputs: true
  navigate: true
---

```{python}
#| label: libraries
#| include: false
import numpy as np
import matplotlib.pyplot as plt
```

## **Question**

**Use [Lagrange interpolation](../../notes/w02/lagrange-interpolation.html) to find a polynomial that passes through the points $(0, -2), (2, 1), (4, 4)$.**

The Lagrange interpolation polynomial for three points $(x_1, y_1), (x_2, y_2),$ and $(x_3, y_3)$ is given by the formula:

$$P(x) = y_1 \frac{(x - x_2)(x - x_3)}{(x_1 - x_2)(x_1 - x_3)} + y_2 \frac{(x - x_1)(x - x_3)}{(x_2 - x_1)(x_2 - x_3)} + y_3 \frac{(x - x_1)(x - x_2)}{(x_3 - x_1)(x_3 - x_2)}$$

The points are:

- $(x_1, y_1) = (0, -2)$
- $(x_2, y_2) = (2, 1)$
- $(x_3, y_3) = (4, 4)$

### **Step-by-step calculation:**

1. **First term** (corresponding to $(x_1, y_1) = (0, -2)$):

$$
-2 \cdot \frac{(x - 2)(x - 4)}{(0 - 2)(0 - 4)} = -2 \cdot \frac{(x - 2)(x - 4)}{(-2)(-4)} = -2 \cdot \frac{(x - 2)(x - 4)}{8} = \frac{-1}{4}(x - 2)(x - 4)
$$

2. **Second term** (corresponding to $(x_2, y_2) = (2, 1)$)

$$
1 \cdot \frac{(x - 0)(x - 4)}{(2 - 0)(2 - 4)} = 1 \cdot \frac{x(x - 4)}{(2)(-2)} = \frac{x(x - 4)}{-4}
$$

3. **Third term** (corresponding to $(x_3, y_3) = (4, 4)$):

$$
4 \cdot \frac{(x - 0)(x - 2)}{(4 - 0)(4 - 2)} = 4 \cdot \frac{x(x - 2)}{(4)(2)} = 4 \cdot \frac{x(x - 2)}{8} = \frac{x(x - 2)}{2}
$$

### **Combine the terms:**

$$
P(x) = \frac{-1}{4}(x - 2)(x - 4) + \frac{x(x - 4)}{-4} + \frac{x(x - 2)}{2}
$$

### **Simplify:**

First term:

$$
\frac{-1}{4}(x - 2)(x - 4) = \frac{-x^2 + 6x - 8}{4}
$$

Second term:

$$
\frac{-x(x - 4)}{4} = \frac{-x^2 + 4x}{4}
$$

Third term:

$$
\frac{x(x - 2)}{2} = \frac{x^2 - 2x}{2}
$$

Combine the terms:

$$
P(x) = \frac{-x^2 + 6x - 8}{4} + \frac{-x^2 + 4x}{4} + \frac{x^2 - 2x}{2}
$$

To combine, first rewrite everything with a denominator of 4:

$$
P(x) = \frac{-x^2 + 6x - 8 - x^2 + 4x}{4} + \frac{x^2 - 2x}{2}
$$

Convert the second term to have a denominator of 4:

$$
P(x) = \frac{-x^2 + 6x - 8 - x^2 + 4x}{4} + \frac{2x^2 - 4x}{4}
$$

Now simplify:

$$
P(x) = \frac{-2x^2 + 10x - 8}{4} + \frac{2x^2 - 4x}{4}
$$

$$
P(x) = \frac{6x - 8}{4} = \frac{3x - 4}{2}
$$

Final polynomial:

$$
P(x) = \frac{3x - 4}{2}
$$

This is the interpolating polynomial that passes through the points $(0, -2)$, $(2, 1)$, and $(4, 4)$.

```{python}
#| label: Graph
#| code-summary: Create graph with resulting polynomial

# Define the Lagrange interpolating polynomial
def lagrange_polynomial(x):
    return (3 * x - 4) / 2

# Create an array of x values from -1 to 5 for the graph
x_values = np.linspace(-1, 5, 400)

# Compute the corresponding y values using the polynomial function
y_values = lagrange_polynomial(x_values)

# Plot the polynomial curve
plt.figure(figsize=(8, 6))
plt.plot(x_values, y_values, label="P(x) = (3x - 4) / 2", color="blue")

# Plot the given points (0,-2), (2,1), (4,4)
data_points_x = [0, 2, 4]
data_points_y = [-2, 1, 4]
plt.scatter(data_points_x, data_points_y, color="red", label="Data Points", zorder=5)

# Add labels, title, and legend
plt.title("Lagrange Interpolating Polynomial")
plt.xlabel("x")
plt.ylabel("P(x)")

# Set x and y ticks to have increments of 1
plt.xticks(np.arange(-1, 6, 1))
plt.yticks(np.arange(-4, 5, 1))

plt.axhline(0, color='black',linewidth=0.5)
plt.axvline(0, color='black',linewidth=0.5)
plt.grid(True)
plt.legend()

# Show the plot
plt.show()
```
