---
title: 'Exercise 3.1.1a (C3-P1)'
subtitle: 'MATH411'
author: 'Nathan Lunceford'
format:
  html:
    self-contained: true
    page-layout: full
    toc: true
    toc-depth: 1
    toc-location: right
    number-sections: false
    html-math-method: katex
    embed-resources: true
    code-fold: true
    code-summary: 'Show the code'
    code-overflow: wrap
    code-copy: hover
    code-tools:
      source: false
      toggle: true
      caption: See code
engine: jupyter
preview:
  port: 3000
  browser: true
  watch-inputs: true
  navigate: true
---

```{python}
#| label: libraries
#| include: false
import numpy as np
import matplotlib.pyplot as plt
```

## **Question**

**Use [Lagrange interpolation](../../notes/w02/lagrange-interpolation.html) to find a polynomial that passes through the points $(0, 1), (2, 3), (3, 0)$.**

The Lagrange interpolation polynomial for three points $(x_1, y_1), (x_2, y_2),$ and $(x_3, y_3)$ is given by the formula:

$$P(x) = y_1 \frac{(x - x_2)(x - x_3)}{(x_1 - x_2)(x_1 - x_3)} + y_2 \frac{(x - x_1)(x - x_3)}{(x_2 - x_1)(x_2 - x_3)} + y_3 \frac{(x - x_1)(x - x_2)}{(x_3 - x_1)(x_3 - x_2)}$$

The points are:

- $(x_1, y_1) = (0, 1)$
- $(x_2, y_2) = (2, 3)$
- $(x_3, y_3) = (3, 0)$

### **Step-by-step calculation:**

1. **First term** (corresponding to $(x_1, y_1) = (0, 1)$):

$$
1 \cdot \frac{(x - 2)(x - 3)}{(0 - 2)(0 - 3)} = 1 \cdot \frac{(x - 2)(x - 3)}{(-2)(-3)} = \frac{(x - 2)(x - 3)}{6}
$$

2. **Second term** (corresponding to $(x_2, y_2) = (2, 3)$)

$$
3 \cdot \frac{(x - 0)(x - 3)}{(2 - 0)(2 - 3)} = 3 \cdot \frac{(x)(x - 3)}{(2)(-1)} = -\frac{3x(x - 3)}{2}
$$

3. **Third term** (corresponding to $(x_3, y_3) = (3, 0)$):

$$
0 \cdot \frac{(x - 0)(x - 2)}{(3 - 0)(3 - 2)} = 0
$$

### **Combine the terms:**

$$
P(x) = \frac{(x - 2)(x - 3)}{6} - \frac{3x(x - 3)}{2}
$$

### **Simplify:**

First term:

$$
\frac{(x - 2)(x - 3)}{6} = \frac{x^2 - 5x + 6}{6}
$$

Second term:

$$
-\frac{3x(x - 3)}{2} = -\frac{3(x^2 - 3x)}{2} = -\frac{3x^2}{2} + \frac{9x}{2}
$$

Now, combine these two terms:

$$
P(x) = \frac{x^2 - 5x + 6}{6} - \left(\frac{3x^2}{2} - \frac{9x}{2}\right)
$$

To combine, first rewrite everything with a denominator of 6:

$$
P(x) = \frac{x^2 - 5x + 6}{6} - \frac{9x^2 - 27x}{6}
$$

Now simplify:

$$
P(x) = \frac{x^2 - 5x + 6 - 9x^2 + 27x}{6}
$$

$$
P(x) = \frac{-8x^2 + 22x + 6}{6}
$$

This is the final polynomial:

$$
P(x) = \frac{-4x^2 + 11x + 3}{3}
$$

This is the interpolating polynomial that passes through the points $(0, 1)$, $(2, 3)$, and $(3, 0)$.

```{python}
#| label: Graph
#| code-summary: Create graph with resulting polynomial

# Define the Lagrange interpolating polynomial
def lagrange_polynomial(x):
    return (-4 * x**2 + 11 * x + 3) / 3

# Create an array of x values from -1 to 4 for the graph
x_values = np.linspace(-1, 4, 400)

# Compute the corresponding y values using the polynomial function
y_values = lagrange_polynomial(x_values)

# Plot the polynomial curve
plt.figure(figsize=(8, 6))
plt.plot(x_values, y_values, label="P(x) = (-4x^2 + 11x + 3) / 3", color="blue")

# Plot the given points (0,1), (2,3), (3,0)
data_points_x = [0, 2, 3]
data_points_y = [1, 3, 0]
plt.scatter(data_points_x, data_points_y, color="red", label="Data Points", zorder=5)

# Add labels, title, and legend
plt.title("Lagrange Interpolating Polynomial")
plt.xlabel("x")
plt.ylabel("P(x)")

# Set x and y ticks to have increments of 1
plt.xticks(np.arange(-1, 5, 1))
plt.yticks(np.arange(-6, 7, 1))

plt.axhline(0, color='black',linewidth=0.5)
plt.axvline(0, color='black',linewidth=0.5)
plt.grid(True)
plt.legend()

# Show the plot
plt.show()

```
